{
  "@context": {
    "schema": "http://schema.org/",
    "rdf": "http://www.w3.org/1999/02/22-rdf-syntax-ns#",
    "rdfs": "http://www.w3.org/2000/01/rdf-schema#",
    "bs": "https:/bioschemas.org/terms/",
    "codemeta": "https://w3id.org/codemeta/",
    "m4ml": "https://discovery.biothings.io/view/m4ml/"
  },
  "@graph": [
    {
      "@id": "m4ml:MLSoftwareSourceCode",
      "@type": "rdfs:Class",
      "rdfs:comment": "A software source code used to create a machine learning model.",
      "rdfs:label": "MLSoftwareSourceCode",
      "rdfs:subClassOf": {
        "@id": "schema:SoftwareSourceCode"
      },
      "schemaVersion": [
        "https://schema.org/docs/releases.html#v23.0"
      ]
    },
    {
      "@id": "m4ml:MLSoftwareApplication",
      "@type": "rdfs:Class",
      "rdfs:comment": "A software application used to create a machine learning model.",
      "rdfs:label": "MLSoftwareApplication",
      "rdfs:subClassOf": {
        "@id": "schema:SoftwareApplication"
      },
      "schemaVersion": [
        "https://schema.org/docs/releases.html#v23.0"
      ]
    },
    {
      "@id": "m4ml:MLModel",
      "@type": "rdfs:Class",
      "rdfs:comment": "An 'executable' ML model that could be used by third-parties for direct use, deployment, fine-tuning, transfer learning, etc.",
      "rdfs:label": "MLModel",
      "rdfs:subClassOf": {
        "@id": "schema:SoftwareApplication"
      },
      "schemaVersion": [
        "https://schema.org/docs/releases.html#v23.0"
      ]
    },
    {
      "@id": "m4ml:MLModelValidationAction",
      "@type": "rdfs:Class",
      "rdfs:comment": "An external validation done for an ML model.",
      "rdfs:label": "MLModelValidationAction",
      "rdfs:subClassOf": {
        "@id": "schema:Action"
      },
      "schemaVersion": [
        "https://schema.org/docs/releases.html#v23.0"
      ]
    },

    {
      "@id": "m4ml:deployedAt",
      "@type": "rdf:Property",
      "rdfs:comment": "Platform, website, webservice or similar where this ML model has been deployed. There could be deployments that this ML model is not aware of (e.g., done by third-parties).",
      "rdfs:label": "deployedAt",
      "schema:domainIncludes": [
        {
          "@id": "m4ml:MLModel"
        }
      ],
      "schema:rangeIncludes": [
         {
           "@id": "schema:Thing"
         }
      ]
    },
    {
      "@id": "m4ml:evaluationMetric",
      "@type": "rdf:Property",
      "rdfs:comment": "Evaluation metrics used by the software for the training process. As the same software can be used for multiple runs (e.g., to find the  best performing model), no actual values for the evaluation metrics should be specified here, only the metrics themselves. For instance precision (a positive number).",
      "rdfs:label": "evaluationMetric",
      "schema:domainIncludes": [
        {
          "@id": "m4ml:MLSoftwareSourceCode"
        },
        {
          "@id": "m4ml:MLSoftwareApplication"
        }
      ],
      "schema:rangeIncludes": [
        {
          "@id": "bs:FormalParameter"
        },
        {
          "@id": "schema:PropertyValue"
        }
      ]
    },
    {
      "@id": "m4ml:evaluationMetricValue",
      "@type": "rdf:Property",
      "rdfs:comment": "Evaluation metric values obtained when creating this ML model. There should be a correspondence with the evaluation metrics declared by the ML software used to create this ML model.",
      "rdfs:label": "evaluationMetricValue",
      "schema:domainIncludes": [
        {
          "@id": "m4ml:MLModel"
        },
        {
          "@id": "m4ml:MLModelValidationAction"
        }
      ],
      "schema:rangeIncludes": [
        {
          "@id": "schema:PropertyValue"
        }
      ]
    },
    {
      "@id": "m4ml:externalValidation",
      "@type": "rdf:Property",
      "rdfs:comment": "A validation action using this ML model with an external validation dataset (e.g., when new datasets are produced from experiments and were not used as part of the learning process of this ML model). There could be external validations that this ML model is not aware of (e.g., done by third-parties).",
      "rdfs:label": "externalValidation",
      "schema:domainIncludes": [
        {
          "@id": "m4ml:MLModel"
        }
      ],
      "schema:rangeIncludes": [
        {
          "@id": "m4ml:MLModelValidationAction"
        }
      ]
    },
    {
      "@id": "m4ml:fineTunedBy",
      "@type": "rdf:Property",
      "rdfs:comment": "ML Software fine-tuning this ML model.",
      "rdfs:label": "fineTunedBy",
      "schema:domainIncludes": [
        {
          "@id": "m4ml:MLModel"
        }
      ],
      "schema:rangeIncludes": [
         {
           "@id": "m4ml:MLSoftwareSourceCode"
         },
         {
          "@id": "m4ml:MLSoftwareApplication"
        }
      ]
    },
    {
      "@id": "m4ml:generatedBy",
      "@type": "rdf:Property",
      "rdfs:comment": "ML software used to create this ML model.",
      "rdfs:label": "generatedBy",
      "schema:domainIncludes": [
        {
          "@id": "m4ml:MLModel"
        }
      ],
      "schema:rangeIncludes": [
         {
           "@id": "m4ml:MLSoftwareSourceCode"
         },
         {
          "@id": "m4ml:MLSoftwareApplication"
        }
      ]
    },
    {
      "@id": "m4ml:hyperparameter",
      "@type": "rdf:Property",
      "rdfs:comment": "Hyperparameters used by the software for the training process. As the same software can be used for multiple runs (e.g., to find the  best performing model), no actual values for the hyperparameters should be specified here, only the hyperparameters themselves. For instance windowSize (a number) or kernelSize (a number).",
      "rdfs:label": "hyperparameter",
      "schema:domainIncludes": [
        {
          "@id": "m4ml:MLSoftwareSourceCode"
        },
        {
          "@id": "m4ml:MLSoftwareApplication"
        }
      ],
      "schema:rangeIncludes": [
        {
          "@id": "bs:FormalParameter"
        },
        {
          "@id": "schema:PropertyValue"
        }
      ]
    },
    {
      "@id": "m4ml:hyperparameterValue",
      "@type": "rdf:Property",
      "rdfs:comment": "Hyperparameter values used to create this ML model. There should be a correspondence with the hyperparameters declared by the ML software used to create this ML model.",
      "rdfs:label": "hyperparameterValue",
      "schema:domainIncludes": [
        {
          "@id": "m4ml:MLModel"
        }
      ],
      "schema:rangeIncludes": [
         {
           "@id": "schema:PropertyValue"
         }
      ]
    },    
    {
      "@id": "m4ml:mlAlgorithm",
      "@type": "rdf:Property",
      "rdfs:comment": "ML algorithm used to solve the task. For instance logistic regression or random forests.",
      "rdfs:label": "mlAlgorithm",
      "schema:domainIncludes": [
        {
          "@id": "m4ml:MLSoftwareSourceCode"
        },
        {
          "@id": "m4ml:MLSoftwareApplication"
        },
        {
          "@id": "m4ml:MLModel"
        }
      ],
      "schema:rangeIncludes": [
        {
          "@id": "schema:Text"
        },
        {
          "@id": "schema:DefinedTerm"
        }
      ]
    },
    {
      "@id": "m4ml:mlTask",
      "@type": "rdf:Property",
      "rdfs:comment": "ML task addressed by this Ml software or model. For instance binary classification.",
      "rdfs:label": "mlTask",
      "schema:domainIncludes": [
        {
          "@id": "m4ml:MLSoftwareSourceCode"
        },
        {
          "@id": "m4ml:MLSoftwareApplication"
        },
        {
          "@id": "m4ml:MLModel"
        }
      ],
      "schema:rangeIncludes": [
        {
          "@id": "schema:Text"
        },
        {
          "@id": "schema:DefinedTerm"
        }
      ]
    },
    {
      "@id": "m4ml:optimizedFor",
      "@type": "rdf:Property",
      "rdfs:comment": "AI-ready dataset (after pre-processing) used by the ML software for the training and optimization of this ML model.",
      "rdfs:label": "optimizedFor",
      "schema:domainIncludes": [
        {
          "@id": "m4ml:MLModel"
        }
      ],
      "schema:rangeIncludes": [
         {
           "@id": "schema:Dataset"
         }
      ]
    },
    {
      "@id": "m4ml:retrainedBy",
      "@type": "rdf:Property",
      "rdfs:comment": "ML software used to re-train this ML model.",
      "rdfs:label": "retrainedBy",
      "schema:domainIncludes": [
        {
          "@id": "m4ml:MLModel"
        }
      ],
      "schema:rangeIncludes": [
         {
           "@id": "m4ml:MLSoftwareSourceCode"
         },
         {
          "@id": "m4ml:MLSoftwareApplication"
        }
      ]
    },
    {
      "@id": "m4ml:validatesMLModel",
      "@type": "rdf:Property",
      "rdfs:comment": "ML model validated by this validation action.",
      "rdfs:label": "validatesMLModel",
      "schema:domainIncludes": [
        {
          "@id": "m4ml:MLModelValidationAction"
        }
      ],
      "schema:rangeIncludes": [
         {
           "@id": "m4ml:MLModel"
         }
      ]
    },
    {
      "@id": "m4ml:validationData",
      "@type": "rdf:Property",
      "rdfs:comment": "AI-ready dataset (after pre-processing) used by the ML validation action to perform an external validation with an unseen dataset.",
      "rdfs:label": "validationData",
      "schema:domainIncludes": [
        {
          "@id": "m4ml:MLModelValidationAction"
        }
      ],
      "schema:rangeIncludes": [
         {
           "@id": "schema:Dataset"
         }
      ]
    }
  ]
}
